Ensure that all transformations are parametric over EEnvFlags, even if the erasure uses the concrete all_env_flags
This is preparation to remove tVar/tEvar from all_env_flags as those are not typeable, which has implications down the line in the correctness statement for CertiRocq.

erasure-plugin/theories/ETransform.v
@@ -737,7 +737,7 @@ Proof.
 Qed.
 
 Program Definition remove_params_optimization {fl : EWcbvEval.WcbvFlags} {wcon : EWcbvEval.with_constructor_as_block = false}
-  (efl := all_env_flags):
+  (efl : EEnvFlags) (has_app : has_tApp) (cstrs : cstr_as_blocks = false) :
   Transform.t _ _ EAst.term EAst.term _ _ (eval_eprogram_env fl) (eval_eprogram fl) :=
   {| name := "stripping constructor parameters (using a view)";
     transform p pre := ERemoveParams.strip_program p;
@@ -745,7 +745,7 @@ Program Definition remove_params_optimization {fl : EWcbvEval.WcbvFlags} {wcon :
     post p := wf_eprogram (switch_no_params efl) p /\ EEtaExpanded.expanded_eprogram_cstrs p;
     obseq p hp p' v v' := v' = (ERemoveParams.strip p.1 v) |}.
 Next Obligation.
-  move=> fl wcon efl [Σ t] [wfp etap].
+  move=> fl wcon efl has_app cstrs [Σ t] [wfp etap].
   simpl.
   cbn -[ERemoveParams.strip] in *.
   split. now eapply ERemoveParams.strip_program_wf.
@@ -753,19 +753,19 @@ Next Obligation.
 Qed.
 
 Next Obligation.
-  red. move=> ? wcon [Σ t] /= v [[wfe wft] etap] [ev].
-  unshelve eapply ERemoveParams.strip_eval in ev; eauto.
-  eexists; split => /= //. now sq. cbn in *.
-  now move/andP: etap.
-  now eapply wellformed_closed_env.
-  now eapply wellformed_closed.
-  now move/andP: etap.
+  red. move=> ? wcon efl hasapp cstrs [Σ t] /= v [[wfe wft] etap] [ev].
+  unshelve eapply ERemoveParams.strip_eval in ev; cbn -[strip] in *; eauto.
+  eexists; split => /= //.
+  - now sq.
+  - now move/andP: etap.
+  - now eapply wellformed_closed_env.
+  - now move/andP: etap.
 Qed.
 
 #[global]
 Instance remove_params_extends {fl : EWcbvEval.WcbvFlags}  {wcon : EWcbvEval.with_constructor_as_block = false}
-  (efl := all_env_flags):
-  TransformExt.t (remove_params_optimization (wcon:=wcon)) (fun p p' => extends p.1 p'.1) (fun p p' => extends p.1 p'.1).
+  (efl : EEnvFlags) (has_app : has_tApp) (cstrs : cstr_as_blocks = false) :
+  TransformExt.t (remove_params_optimization (fl := fl) (wcon:=wcon) efl has_app cstrs) (fun p p' => extends p.1 p'.1) (fun p p' => extends p.1 p'.1).
 Proof.
   red. intros p p' pr pr' ext. rewrite /transform /= /strip_program.
   red. cbn -[strip_env strip]. eapply strip_extends_env => //. apply pr. apply pr'.
@@ -773,8 +773,8 @@ Qed.
 
 #[global]
 Instance remove_params_extends' {fl : EWcbvEval.WcbvFlags}  {wcon : EWcbvEval.with_constructor_as_block = false}
-  (efl := all_env_flags):
-  TransformExt.t (remove_params_optimization (wcon:=wcon)) extends_eprogram_env extends_eprogram.
+  (efl : EEnvFlags) (has_app : has_tApp) (cstrs : cstr_as_blocks = false) :
+  TransformExt.t (remove_params_optimization (wcon:=wcon) efl has_app cstrs) extends_eprogram_env extends_eprogram.
 Proof.
   red. intros p p' pr pr' [ext eq]. rewrite /transform /= /strip_program. rewrite eq.
   red. cbn -[strip_env strip]. split. eapply strip_extends_env => //. apply pr. apply pr'.
@@ -782,7 +782,7 @@ Proof.
 Qed.
 
 Program Definition remove_params_fast_optimization {fl : EWcbvEval.WcbvFlags} {wcon : EWcbvEval.with_constructor_as_block = false}
-  (efl := all_env_flags) :
+  (efl : EEnvFlags) (has_app : has_tApp) (cstrs : cstr_as_blocks = false) :
   Transform.t _ _ EAst.term EAst.term _ _ (eval_eprogram_env fl) (eval_eprogram fl) :=
   {| name := "stripping constructor parameters (using accumulators)";
     transform p _ := (ERemoveParams.Fast.strip_env p.1, ERemoveParams.Fast.strip p.1 [] p.2);
@@ -790,31 +790,30 @@ Program Definition remove_params_fast_optimization {fl : EWcbvEval.WcbvFlags} {w
     post p := wf_eprogram (switch_no_params efl) p /\ EEtaExpanded.expanded_eprogram_cstrs p;
     obseq p hp p' v v' := v' = (ERemoveParams.strip p.1 v) |}.
 Next Obligation.
-  move=> fl wcon efl [Σ t] [wfp etap].
+  move=> fl wcon efl has_app cstrs [Σ t] [wfp etap].
   simpl.
   cbn -[ERemoveParams.strip] in *.
   rewrite -ERemoveParams.Fast.strip_fast -ERemoveParams.Fast.strip_env_fast.
   split.
-  now eapply (ERemoveParams.strip_program_wf (Σ, t)).
-  now eapply (ERemoveParams.strip_program_expanded (Σ, t)).
+  now eapply (ERemoveParams.strip_program_wf has_app cstrs (Σ, t)).
+  now eapply (ERemoveParams.strip_program_expanded has_app (Σ, t)).
 Qed.
 
 Next Obligation.
-  red. move=> ? wcon [Σ t] /= v [[wfe wft] etap] [ev].
+  red. move=> ? wcon efl has_app cstrs [Σ t] /= v [[wfe wft] etap] [ev].
   rewrite -ERemoveParams.Fast.strip_fast -ERemoveParams.Fast.strip_env_fast.
   unshelve eapply ERemoveParams.strip_eval in ev; eauto.
   eexists; split => /= //.
   now sq. cbn in *.
   now move/andP: etap.
   now eapply wellformed_closed_env.
-  now eapply wellformed_closed.
   now move/andP: etap.
 Qed.
 
 #[global]
 Instance remove_params_fast_extends {fl : EWcbvEval.WcbvFlags}  {wcon : EWcbvEval.with_constructor_as_block = false}
-  (efl := all_env_flags):
-  TransformExt.t (remove_params_fast_optimization (wcon:=wcon)) (fun p p' => extends p.1 p'.1) (fun p p' => extends p.1 p'.1).
+  (efl : EEnvFlags) (has_app : has_tApp) (cstrs : cstr_as_blocks = false) :
+  TransformExt.t (remove_params_fast_optimization (wcon:=wcon) efl has_app cstrs) (fun p p' => extends p.1 p'.1) (fun p p' => extends p.1 p'.1).
 Proof.
   red. intros p p' pr pr' ext. rewrite /transform /=.
   rewrite -!ERemoveParams.Fast.strip_env_fast.
@@ -823,8 +822,8 @@ Qed.
 
 #[global]
 Instance remove_params_fast_extends' {fl : EWcbvEval.WcbvFlags}  {wcon : EWcbvEval.with_constructor_as_block = false}
-  (efl := all_env_flags):
-  TransformExt.t (remove_params_fast_optimization (wcon:=wcon)) extends_eprogram_env extends_eprogram.
+  (efl : EEnvFlags) (has_app : has_tApp) (cstrs : cstr_as_blocks = false) :
+  TransformExt.t (remove_params_fast_optimization (wcon:=wcon) efl has_app cstrs) extends_eprogram_env extends_eprogram.
 Proof.
   red. intros p p' pr pr' [ext eq]. rewrite /transform /=. rewrite eq.
   rewrite -!ERemoveParams.Fast.strip_env_fast -!ERemoveParams.Fast.strip_fast.
@@ -877,7 +876,10 @@ Qed.
 
 From MetaRocq.Erasure Require Import EInlineProjections.
 
-Program Definition inline_projections_optimization {fl : WcbvFlags} {wcon : EWcbvEval.with_constructor_as_block = false} (efl := switch_no_params all_env_flags)
+Program Definition inline_projections_optimization {fl : WcbvFlags} {wcon : EWcbvEval.with_constructor_as_block = false} {efl : EEnvFlags}
+  (cstrs : cstr_as_blocks = false)
+  (no_pars : has_cstr_params = false)
+  {has_app : has_tApp}
   {hastrel : has_tRel} {hastbox : has_tBox} :
   Transform.t _ _ EAst.term EAst.term _ _ (eval_eprogram_env fl) (eval_eprogram fl) :=
   {| name := "primitive projection inlining";
@@ -887,31 +889,37 @@ Program Definition inline_projections_optimization {fl : WcbvFlags} {wcon : EWcb
     obseq p hp p' v v' := v' = EInlineProjections.optimize p.1 v |}.
 
 Next Obligation.
-  move=> fl wcon efl hastrel hastbox [Σ t] [wfp etap].
+  move=> fl wcon efl cstrs no_pars hasapp hastrel hastbox [Σ t] [wfp etap].
   cbn in *. split.
   - now eapply optimize_program_wf.
   - now eapply optimize_program_expanded.
 Qed.
 Next Obligation.
-  red. move=> fl wcon hastrel hastbox [Σ t] /= v [wfe wft] [ev].
+  red. move=> fl wcon efl cstrs no_pars hasapp hastrel hastbox [Σ t] /= v [wfe wft] [ev].
   eapply EInlineProjections.optimize_correct in ev; eauto.
   eexists; split => //. red. sq; auto. cbn. apply wfe.
   cbn. eapply wfe. Unshelve. auto.
 Qed.
 
 #[global]
-Instance inline_projections_optimization_extends {fl : WcbvFlags} {wcon : EWcbvEval.with_constructor_as_block = false} (efl := switch_no_params all_env_flags)
+Instance inline_projections_optimization_extends {fl : WcbvFlags} {wcon : EWcbvEval.with_constructor_as_block = false} {efl : EEnvFlags}
+  (cstrs : cstr_as_blocks = false)
+  (no_pars : has_cstr_params = false)
+  {has_app : has_tApp}
   {hastrel : has_tRel} {hastbox : has_tBox} :
-  TransformExt.t (inline_projections_optimization (wcon:=wcon) (hastrel := hastrel) (hastbox := hastbox)) (fun p p' => extends p.1 p'.1) (fun p p' => extends p.1 p'.1).
+  TransformExt.t (inline_projections_optimization (wcon:=wcon) cstrs no_pars (has_app := has_app) (hastrel := hastrel) (hastbox := hastbox)) (fun p p' => extends p.1 p'.1) (fun p p' => extends p.1 p'.1).
 Proof.
   red. intros p p' pr pr' ext. rewrite /transform /= /optimize_program /=.
   eapply optimize_extends_env => //. apply pr. apply pr'.
 Qed.
 
 #[global]
-Instance inline_projections_optimization_extends' {fl : WcbvFlags} {wcon : EWcbvEval.with_constructor_as_block = false} (efl := switch_no_params all_env_flags)
+Instance inline_projections_optimization_extends' {fl : WcbvFlags} {wcon : EWcbvEval.with_constructor_as_block = false} {efl : EEnvFlags}
+  (cstrs : cstr_as_blocks = false)
+  (no_pars : has_cstr_params = false)
+  {has_app : has_tApp}
   {hastrel : has_tRel} {hastbox : has_tBox} :
-  TransformExt.t (inline_projections_optimization (wcon:=wcon) (hastrel := hastrel) (hastbox := hastbox)) extends_eprogram_env extends_eprogram.
+  TransformExt.t (inline_projections_optimization (wcon:=wcon) cstrs no_pars (has_app := has_app) (hastrel := hastrel) (hastbox := hastbox)) extends_eprogram_env extends_eprogram.
 Proof.
   red. intros p p' pr pr' [ext eq]. rewrite /transform /= /optimize_program /=. split.
   eapply optimize_extends_env => //. apply pr. apply pr'.
@@ -997,7 +1005,7 @@ Definition efl_coind_to_ind (efl : EEnvFlags) :=
     |}.
 
 Program Definition coinductive_to_inductive_transformation (efl : EEnvFlags)
-  {has_app : has_tApp} {has_box : has_tBox} {has_rel : has_tRel} {has_pars : has_cstr_params = false}
+  {has_app : has_tApp} {has_rel : has_tRel} {has_pars : has_cstr_params = false}
   {has_cstrblocks : cstr_as_blocks = true} :
   Transform.t _ _ EAst.term EAst.term _ _
     (eval_eprogram_env block_wcbv_flags) (eval_eprogram block_wcbv_flags) :=
@@ -1008,13 +1016,13 @@ Program Definition coinductive_to_inductive_transformation (efl : EEnvFlags)
     obseq p hp p' v v' := v' = ECoInductiveToInductive.trans p.1 v |}.
 
 Next Obligation.
-  move=> efl hasapp hasbox hasrel haspars hascstrs [Σ t] [wftp wft].
+  move=> efl hasapp hasrel haspars hascstrs [Σ t] [wftp wft].
   cbn in *. eapply ECoInductiveToInductive.trans_program_wf; eauto. split => //.
   - apply ECoInductiveToInductive.trust_cofix.
   - apply ECoInductiveToInductive.trust_cofix.
 Qed.
 Next Obligation.
-  red. move=> efl hasapp hasbox hasrel haspars hascstrs [Σ t] /= v [wfe1 wfe2] [ev].
+  red. move=> efl hasapp hasrel haspars hascstrs [Σ t] /= v [wfe1 wfe2] [ev].
   eexists. split; [ | eauto].
   econstructor.
   cbn -[transform_blocks].
@@ -1025,9 +1033,9 @@ Qed.
 
 #[global]
 Instance coinductive_to_inductive_transformation_ext (efl : EEnvFlags)
-  {has_app : has_tApp} {has_rel : has_tRel} {has_box : has_tBox} {has_pars : has_cstr_params = false} {has_cstrblocks : cstr_as_blocks = true} :
+  {has_app : has_tApp} {has_rel : has_tRel} {has_pars : has_cstr_params = false} {has_cstrblocks : cstr_as_blocks = true} :
   TransformExt.t (coinductive_to_inductive_transformation efl (has_app := has_app) (has_rel := has_rel)
-    (has_box := has_box) (has_pars := has_pars) (has_cstrblocks := has_cstrblocks))
+    (has_pars := has_pars) (has_cstrblocks := has_cstrblocks))
     (fun p p' => extends p.1 p'.1) (fun p p' => extends p.1 p'.1).
 Proof.
   red. intros p p' pr pr' ext. rewrite /transform /=.
@@ -1038,7 +1046,7 @@ Qed.
 Instance coinductive_to_inductive_transformation_ext' (efl : EEnvFlags)
   {has_app : has_tApp} {has_rel : has_tRel} {has_box : has_tBox} {has_pars : has_cstr_params = false} {has_cstrblocks : cstr_as_blocks = true} :
   TransformExt.t (coinductive_to_inductive_transformation efl (has_app := has_app) (has_rel := has_rel)
-    (has_box := has_box) (has_pars := has_pars) (has_cstrblocks := has_cstrblocks))
+    (has_pars := has_pars) (has_cstrblocks := has_cstrblocks))
     extends_eprogram_env extends_eprogram.
 Proof.
   red. intros p p' pr pr' ext. rewrite /transform /=.
